use alternative version of COMB

thys/List_Update/Comb.thy
@@ -1,5 +1,5 @@
 theory Comb
-imports TS BIT_2comp_on2 BIT_pairwise
+imports TS BIT_2comp_on2 BIT_pairwise Sum_Distribution
 begin
 
 
@@ -7,723 +7,325 @@ begin
     state of TS: nat list       history
 *)
 
+section "Definition of Comb"
 
-
-
-datatype CombState = CBit "bool list * nat list" | CTs "nat list" 
+type_synonym CombState = "(bool list * nat list) + (nat list)" 
                           
-fun COMB_init :: "nat list \<Rightarrow> (nat state, CombState) alg_on_init" where
-  "COMB_init h init = do {
+definition COMB_init :: "nat list \<Rightarrow> (nat state, CombState) alg_on_init" where
+  "COMB_init h init = 
+        Sum_pmf 0.8 (fst BIT init) (fst (embed (rTS h)) init)"
+
+lemma COMB_init[simp]: "COMB_init h init =
+                do {
                     (b::bool) \<leftarrow> (bernoulli_pmf 0.8);
                     (xs::bool list) \<leftarrow> Prob_Theory.bv (length init);
-                    return_pmf (if b then CBit (xs, init) else CTs h)
-                  }"
-  
+                    return_pmf (if b then Inl (xs, init) else Inr h)
+                  }" 
+ apply(simp add: bind_return_pmf COMB_init_def BIT_init_def rTS_def
+              bind_assoc_pmf )
+ unfolding map_pmf_def Sum_pmf_def
+ apply(simp add: if_distrib bind_return_pmf bind_assoc_pmf )
+    apply(rule bind_pmf_cong) 
+     by(auto simp add: bind_return_pmf bind_assoc_pmf)
+
 definition COMB_step :: "(nat state, CombState, nat, answer) alg_on_step" where
-"COMB_step s q = (case snd s of CBit b \<Rightarrow> map_pmf (\<lambda>((a,b),c). ((a,b),CBit c)) (BIT_step (fst s, b) q)
-                              | CTs b \<Rightarrow> map_pmf (\<lambda>((a,b),c). ((a,b),CTs c)) (return_pmf (TS_step_d (fst s, b) q)))"
+"COMB_step s q = (case snd s of Inl b \<Rightarrow> map_pmf (\<lambda>((a,b),c). ((a,b),Inl c)) (BIT_step (fst s, b) q)
+                              | Inr b \<Rightarrow> map_pmf (\<lambda>((a,b),c). ((a,b),Inr c)) (return_pmf (TS_step_d (fst s, b) q)))"
             
 definition "COMB h = (COMB_init h, COMB_step)"
+ 
 
-term "config'' (embed (rTS h)) qs init i"
-term "config'' BIT qs init i"
-lemma configCOMB: "i \<le> length qs \<Longrightarrow> config'' (COMB h) qs init i = do {
-                    (b::bool) \<leftarrow> (bernoulli_pmf 0.8); 
-                    (b1,b2) \<leftarrow>  (config'' BIT qs init i);
-                    (t1,t2) \<leftarrow>  (config'' (embed (rTS h)) qs init i);
-                    return_pmf (if b then  (b1, CBit b2) else (t1, CTs t2))
-                    }" (is "?Prem \<Longrightarrow> ?LHS = ?RHS i")
-proof (induct i)
-  case 0 
-  show ?case
-  apply(simp add: BIT_init_def COMB_def rTS_def map_pmf_def bind_return_pmf bind_assoc_pmf )
-  apply(rule bind_pmf_cong)
-    apply(simp) 
-    apply(simp only: set_pmf_bernoulli)
-      apply(case_tac x)
-        by(simp_all) 
-next
-  case (Suc n) 
-  from Suc(2) show ?case apply(simp add: take_Suc_conv_app_nth)
-    apply(subst config'_rand_append)
-    apply(subst Suc(1))
-      apply(simp)
-      apply(simp add: bind_return_pmf bind_assoc_pmf split_def config'_rand_append)
-        apply(rule bind_pmf_cong)
-          apply(simp) 
-          apply(simp only: set_pmf_bernoulli)
-            apply(case_tac x)
-               by(simp_all add: COMB_def COMB_step_def rTS_def map_pmf_def split_def bind_return_pmf bind_assoc_pmf)
-qed
+section "Comb 1.6-compet on 2 elements"
+ 
+abbreviation "noc == (%x. case x of Inl (s,is) \<Rightarrow> (s,Inl is) | Inr (s,is) \<Rightarrow> (s,Inr is) )"
+abbreviation "con == (%(s,is). case is of Inl is \<Rightarrow> Inl (s,is) | Inr is \<Rightarrow> Inr (s,is) )"
 
+definition "inv_COMB s x i == (\<exists>Da Db. finite (set_pmf Da) \<and> finite (set_pmf Db) \<and>
+      (map_pmf con s) = Sum_pmf 0.8 Da Db \<and> BIT_inv Da x i \<and> TS_inv Db x i)"
 
+lemma noccon: "noc o con = id"
+  apply(rule ext)
+  apply(case_tac x) by(auto simp add: sum.case_eq_if)
+ 
+lemma connoc: "con o noc = id"
+  apply(rule ext)
+  apply(case_tac x) by(auto simp add: sum.case_eq_if) 
 
-lemma BITfin: "x<length qs
-   \<Longrightarrow> finite (set_pmf  (config'_rand BIT  (BIT_init init \<bind>  (\<lambda>is. return_pmf (init, is)))
-                      (take x qs)))"
-apply (induct x)
-  apply(simp add: BIT_init_def bv_finite)
-  by(simp add: take_Suc_conv_app_nth config'_rand_append BIT_step_def)
-  
-lemma TSfin: "x<length qs 
-  \<Longrightarrow> finite (set_pmf (config'_rand (\<lambda>s. return_pmf h, \<lambda>s r. return_pmf (TS_step_d s r))
-                         (return_pmf (init, h))
-                         (take x qs)))" 
-apply (induct x)
-  apply(simp add: BIT_init_def)
-  by(simp add: take_Suc_conv_app_nth config'_rand_append split_def) 
-
-
-lemma T_COMB_split: "T\<^sub>p_on_rand (COMB h) init qs = 0.2 * T\<^sub>p_on_rand (embed (rTS h))  init qs + 0.8 * T\<^sub>p_on_rand BIT  init qs"
-proof -
-  have A: "0.2 * T_on_rand (embed (rTS h))  init qs + 0.8 * T_on_rand BIT  init qs
-      = setsum (%i. 0.2 * T\<^sub>p_on_rand_n (embed (rTS h)) init qs i + 0.8 * T\<^sub>p_on_rand_n BIT  init qs i) {..<length qs}"
-        unfolding T_on_rand_as_sum
-          by(simp only: setsum_right_distrib setsum.distrib) 
-
-
-  show ?thesis unfolding A unfolding T_on_rand_as_sum
-    apply(rule setsum.cong)
-      apply(simp)
-      apply(subst configCOMB)
-        apply(simp)  
-        unfolding rTS_def COMB_def  
-        apply(simp add: bind_assoc_pmf bind_return_pmf split_def ) 
-        apply(subst E_bernoulli3)
-          apply(simp) apply(simp) 
-          using BITfin[of _ qs init] TSfin[of _ qs]
-          apply(simp add: split_def set_pmf_bernoulli BIT_step_def COMB_step_def)
-        unfolding COMB_step_def BIT_init_def map_pmf_def apply(simp add: split_def)
-        apply(simp add: bind_assoc_pmf)
-        by(simp add: bind_return_pmf split_def )  
-qed  
-      
-
-definition "COMB_state h x y i = do {
-                    (b::bool) \<leftarrow> (bernoulli_pmf 0.8);
-                    (l,v)  \<leftarrow> i;
-                    return_pmf (if b then (l, CBit v) else ([x,y], CTs h))
-                  }"
-
-definition "COMB_initial init h x y = do {
-                    (b::bool) \<leftarrow> (bernoulli_pmf 0.8);
-                    (l,v)  \<leftarrow> (type0 init x y);
-                    return_pmf (if b then (l,CBit v) else ([x,y], CTs h))
-                  }"
-
-
-
-lemma config2COMB: "i \<le> length qs \<Longrightarrow> config2 (COMB h) qs (COMB_state h x y BI) i = do {
-                    (b::bool) \<leftarrow> (bernoulli_pmf 0.8); 
-                    (b1,b2) \<leftarrow>  (config2 BIT qs BI i);
-                    (t1,t2) \<leftarrow>  config2 (embed (rTS h)) qs (return_pmf ([x, y], h)) i;
-                    return_pmf (if b then  (b1, CBit b2) else (t1, CTs t2))
-                    }" (is "?Prem \<Longrightarrow> ?LHS = ?RHS i")
-proof (induct i)
-  case 0 
-  show ?case by(simp add: config2_def COMB_state_def bind_return_pmf) 
-next
-  case (Suc n) 
-  from Suc(2) show ?case apply(simp add: config2_def take_Suc_conv_app_nth)
-    apply(subst config'_rand_append)
-    apply(subst Suc(1)[unfolded config2_def])
-      apply(simp)
-      apply(simp add: bind_return_pmf bind_assoc_pmf split_def config'_rand_append)
-        apply(rule bind_pmf_cong)
-          apply(simp) 
-          apply(simp only: set_pmf_bernoulli)
-            apply(case_tac xa)
-               by(simp_all add: COMB_def COMB_step_def rTS_def map_pmf_def split_def bind_return_pmf bind_assoc_pmf)
-qed
-
-
-lemma configCOMB2asd: "config'_rand (COMB h) (COMB_state h x y i) qs  = do {
-                    (b::bool) \<leftarrow> (bernoulli_pmf 0.8); 
-                    (b1,b2) \<leftarrow>  (config'_rand BIT i qs);
-                    (t1,t2) \<leftarrow>  (config'_rand (embed (rTS h)) (return_pmf ([x,y],h)) qs);
-                    return_pmf (if b then  (b1, CBit b2) else (t1, CTs t2))
-                    }" (is "?LHS = ?RHS i")
-proof (induct qs rule: rev_induct)
+lemma obligation1': assumes "map_pmf con s = Sum_pmf (8 / 10) Da Db"
+    shows "config'_rand (COMB h) s qs =
+    map_pmf noc (Sum_pmf (8 / 10) (config'_rand BIT Da qs)
+                     (config'_rand (embed (rTS h)) Db qs))"
+proof (induct qs rule: rev_induct) 
   case Nil
-  show ?case
-  by(simp add: COMB_state_def BIT_init_def COMB_def rTS_def map_pmf_def bind_return_pmf bind_assoc_pmf )
+  have "s = map_pmf noc (map_pmf con s)"
+    by(simp add: pmf.map_comp noccon)
+also
+  from assms have "\<dots> = map_pmf noc (Sum_pmf (8 / 10) Da Db)"
+    by simp
+finally
+  show ?case by simp
 next
-  case (snoc r rs) 
-  show ?case apply(simp add: take_Suc_conv_app_nth)
+  case (snoc q qs) 
+  show ?case apply(simp)
     apply(subst config'_rand_append)
-    apply(subst snoc(1))
-      apply(simp)
-      apply(simp add: bind_return_pmf bind_assoc_pmf split_def config'_rand_append)
+    apply(subst snoc) 
+    apply(simp)
+      unfolding Sum_pmf_def
+      apply(simp add: 
+          bind_assoc_pmf bind_return_pmf COMB_def COMB_step_def)
+      apply(subst config'_rand_append)
+      apply(subst config'_rand_append)
+      apply(simp only: map_pmf_def[where f=noc])
+        apply(simp add: bind_return_pmf bind_assoc_pmf)
         apply(rule bind_pmf_cong)
-          apply(simp) 
-          apply(simp only: set_pmf_bernoulli)
-            apply(case_tac xa)
-               by(simp_all add: COMB_def COMB_step_def rTS_def map_pmf_def split_def bind_return_pmf bind_assoc_pmf)
+          apply(simp)
+         apply(simp only: set_pmf_bernoulli UNIV_bool)
+          apply(auto)
+            apply(simp only: map_pmf_def[where f=Inl])
+            apply(simp add: bind_return_pmf bind_assoc_pmf)
+            apply(rule bind_pmf_cong)
+            apply(simp add: bind_return_pmf bind_assoc_pmf )
+            apply(simp add:  split_def)
+            apply(simp add: bind_return_pmf bind_assoc_pmf map_pmf_def)
+          apply(simp only: map_pmf_def[where f=Inr])
+          apply(simp add: bind_return_pmf bind_assoc_pmf)
+          apply(rule bind_pmf_cong)
+          apply(simp add: bind_return_pmf bind_assoc_pmf )
+          apply(simp add:  split_def)
+          apply(simp add: bind_return_pmf bind_assoc_pmf map_pmf_def rTS_def)
+  done                
+qed 
+  
+lemma obligation1'': 
+    shows "config_rand (COMB h) init qs =
+    map_pmf noc (Sum_pmf (8 / 10) (config_rand BIT init qs)
+                     (config_rand (embed (rTS h)) init qs))"
+apply(rule obligation1')
+  apply(simp add: Sum_pmf_def COMB_def map_pmf_def bind_assoc_pmf bind_return_pmf split_def COMB_init_def del: COMB_init)
+  apply(rule bind_pmf_cong) 
+    by(auto simp add: split_def map_pmf_def bind_return_pmf bind_assoc_pmf)
+                                                
+lemma obligation1: assumes "map_pmf con s = Sum_pmf (8 / 10) Da Db"
+    shows "map_pmf con (config'_rand (COMB []) s qs) = 
+    Sum_pmf (8 / 10) (config'_rand BIT Da qs)
+                     (config'_rand (embed (rTS [])) Db qs)"
+proof -
+  from obligation1'[OF assms] have "map_pmf con (config'_rand (COMB []) s qs)
+      = map_pmf con (map_pmf noc (Sum_pmf (8 / 10) (config'_rand BIT Da qs)
+                     (config'_rand (embed (rTS [])) Db qs)))"
+                by simp
+also
+  have "\<dots> = Sum_pmf (8 / 10) (config'_rand BIT Da qs)
+                     (config'_rand (embed (rTS [])) Db qs)"
+   apply(simp only: pmf.map_comp connoc) by simp
+finally
+  show ?thesis .
 qed
 
- 
-lemma T2_COMB_split: assumes "finite (set_pmf i)"
-  shows "T\<^sub>p_on2 (COMB h) qs (COMB_state h x y i)
-           = 0.2 * T\<^sub>p_on2 (embed (rTS h)) qs (return_pmf ([x,y],h))
-            + 0.8 * T\<^sub>p_on2 BIT qs i"
-proof -
-  have A: "0.2 * T\<^sub>p_on2 (embed (rTS h)) qs (return_pmf ([x,y],h))
-            + 0.8 * T\<^sub>p_on2 BIT qs i 
-      = setsum (\<lambda>j. 0.2 * T_on_rand'_n (embed (rTS h)) (return_pmf ([x, y], h)) qs j
-            + 0.8 * T_on_rand'_n BIT i qs j) {..<length qs}"
-        unfolding  T\<^sub>p_on2_def T_on_n2_def
-          by(simp only: setsum_right_distrib setsum.distrib) 
+lemma BIT_config'_fin: "finite (set_pmf Da) \<Longrightarrow> finite (set_pmf (config'_rand BIT Da qs))"
+apply(induct qs rule: rev_induct)
+  apply(simp) 
+  by(simp add: config'_rand_append BIT_step_def)
 
-  { fix xa 
-    assume "xa<length qs "
-    then have "finite (set_pmf (config'_rand BIT i (take xa qs)))"
-    apply(induct xa)
-      using assms apply(simp)
-      by(simp add: take_Suc_conv_app_nth config'_rand_append split_def BIT_step_def)
-  } note BIT_fin2=this
+lemma TS_config'_fin: "finite (set_pmf Db) \<Longrightarrow> finite (set_pmf (config'_rand (embed (rTS h)) Db qs))"
+apply(induct qs rule: rev_induct)
+  apply(simp) 
+  by(simp add: config'_rand_append rTS_def TS_step_d_def)
 
-  show ?thesis unfolding A unfolding T\<^sub>p_on2_def T_on_n2_def
-    apply(rule setsum.cong)
-      apply(simp)  
-      apply(subst configCOMB2asd)
-        apply(simp)  
-        unfolding rTS_def COMB_def  
-        apply(simp add: bind_assoc_pmf  bind_return_pmf split_def )         
+lemma obligation2: assumes "map_pmf con s = Sum_pmf (8 / 10) Da Db"
+    and "finite (set_pmf Da)"
+    and "finite (set_pmf Db)"
+  shows "T\<^sub>p_on_rand' (COMB []) s qs =
+    2 / 10 * T\<^sub>p_on_rand' (embed (rTS [])) Db qs +
+    8 / 10 * T\<^sub>p_on_rand' BIT Da qs"
+proof (induct qs rule: rev_induct)
+  case (snoc q qs) 
+  have P: "T\<^sub>p_on_rand' (COMB []) (config'_rand (COMB []) s qs) [q]
+      = 2 / 10 * T\<^sub>p_on_rand' (embed (rTS [])) (config'_rand (embed (rTS [])) Db qs) [q] +
+          8 / 10 * T\<^sub>p_on_rand' BIT (config'_rand BIT Da qs) [q]"
+    apply(subst obligation1'[OF assms(1)])
+    unfolding Sum_pmf_def
+      apply(simp)
+      apply(simp only: map_pmf_def[where f=noc])
+      apply(simp add: bind_assoc_pmf )
         apply(subst E_bernoulli3)
-          apply(simp) apply(simp) 
-          using BIT_fin2 TSfin[of _ qs]
-          apply(simp add: split_def set_pmf_bernoulli BIT_step_def COMB_step_def)
-        unfolding COMB_step_def BIT_init_def map_pmf_def apply(simp add: split_def)
-        apply(simp add: bind_assoc_pmf)
-        by(simp add: bind_return_pmf split_def )   
-qed  
-
-
-
-definition "pre_inv_COMB init x y h = (h=[] \<or> (\<exists>hs. h = [x,x]@hs))"
-definition "inv_COMB init qs x y h = (inv_BIT init qs x y \<and> inv_TS qs x y h)"
-
-lemma TS_help: "T\<^sub>p_on_rand (embed (rTS h)) [x,y] qs
-      = T\<^sub>p_on2 (embed (rTS h)) qs (return_pmf ([x,y],h))" 
-    unfolding T\<^sub>p_on2_def T_on_n2_def T_on_rand_as_sum rTS_def by(simp add: bind_return_pmf)
- 
-lemma D: "qs \<in> Lxx x y \<Longrightarrow> x \<noteq> y \<Longrightarrow>
-      pre_inv_COMB init x y h \<Longrightarrow> init \<in> {[x, y], [y, x]} \<Longrightarrow>
-      T\<^sub>p_on2 (COMB h) qs (COMB_state h x y (type0 init x y)) \<le> 1.6 * T\<^sub>p [x, y] qs (OPT2 qs [x, y])
-       \<and> inv_COMB init qs x y h"
-proof (rule LxxI[where P="(\<lambda>x y qs.  T\<^sub>p_on2 (COMB h) qs (COMB_state h x y (type0 init x y)) \<le> 1.6 * T\<^sub>p [x, y] qs (OPT2 qs [x, y]) \<and>
-                                   inv_COMB init qs x y h)"], goal_cases)
-  case 1
-  from 1(3)[unfolded pre_inv_COMB_def inv_TS_def] obtain x' y' where "x'=x" and "y'=y" 
-      and h: "h=[] \<or> (\<exists>hs. h = [x, x] @ hs)" unfolding s_TS_def by(auto)
-  from ts_d[OF 1(1,2) h 1(5)]
-  have "real (T_TS [x, y] h qs) = 0"
-      and TS_inv: "inv_TS qs x y h"  by auto
-  then have "T\<^sub>p_on_rand (embed (rTS h)) [x,y] qs = 0" using T_TS_T_on T_on_embed by metis
-  then have TS: "T\<^sub>p_on2 (embed (rTS h)) qs (return_pmf ([x,y],h)) = 0" using TS_help by metis
-  have BIT: "T\<^sub>p_on2 BIT qs (type0 init x y)  = 0" apply(rule BIT_d) using 1 by auto
-  have BIT_inv: "inv_BIT init qs x y" unfolding inv_BIT_def apply(rule BIT_d_config) using 1 by auto
-
-  have "T\<^sub>p_on2 (COMB h) qs (COMB_state h x y (type0 init x y)) 
-      = 0.2 * T\<^sub>p_on2 (embed (rTS h)) qs (return_pmf ([x,y],h))
-            + 0.8 * T\<^sub>p_on2 BIT qs (type0 init x y)"
-    apply(rule T2_COMB_split) 
-      by(simp add: type0_def)
-  also have "\<dots> = 0" using TS BIT by simp
-  also have "\<dots> \<le> 1.6 * T\<^sub>p [x, y] qs (OPT2 qs [x, y])" by simp
-  finally show ?case unfolding inv_COMB_def using BIT_inv TS_inv by auto
-next
-  case 2  
-  obtain u v where uu: "u \<in> lang (Plus (Atom x) One)"
-    and vv: "v \<in> lang (seq[Times (Atom y) (Atom x), Star (Times (Atom y) (Atom x)), Atom y, Atom y])"
-    and qsuv: "qs = u @ v" 
-    using 2
-    by (auto simp: conc_def) 
-
-  have lenv: "length v > 1 \<and> last v = y \<and> v\<noteq>[]"
-  proof -
-    from vv have "v \<in> ({[y]} @@ {[x]}) @@ star({[y]} @@ {[x]}) @@ {[y]} @@ {[y]}" by(simp add: conc_assoc)
-    then obtain p q r where pqr: "v=p@q@r" and "p\<in>({[y]} @@ {[x]})"
-              and q: "q \<in> star ({[y]} @@ {[x]})" and "r \<in>{[y]} @@ {[y]}" by (metis concE)
-    then have rr: "p = [y,x]" "r=[y,y]" by auto
-    with pqr have a: "length v = 4+length q" by auto
-
-    have "last v = last r" using pqr rr by auto
-    then have c: "last v = y" using rr by auto
-    with a show ?thesis by auto
-  qed
-
-
-  (* TS *)  
-  from 2(3)[unfolded pre_inv_COMB_def inv_TS_def] obtain x' y' where "x'=x" and "y'=y" 
-      and h: "h=[] \<or> (\<exists>hs. h = [x, x] @ hs)" unfolding s_TS_def by(auto)
-  from TS_xr[OF 2(2) uu h]
-  have  TS_1: "T_TS [x, y] h (u@v) = T_TS [x,y] (rev u @ h) v"
-    and TS_2: "(\<exists>hs. (rev u @ h) = [x, x] @ hs) \<or> (rev u @ h) = [x] \<or> (rev u @ h)=[]" by auto
-  from ts_b[OF 2(2) vv TS_2]
-  have  TS_3: "T_TS [x, y] (rev u @ h) v = (length v - 2)"
-         and  inv1: "s_TS [x,y] (rev u @ h) v (length v) = [y,x]"
-         and  inv2: "(\<exists>hs. (rev v @ (rev u @ h)) = [y,y]@hs)" by auto
-  have "T\<^sub>p_on_rand (embed (rTS h))  [x,y] qs = (length v - 2)"
-    unfolding  qsuv using T_on_embed T_TS_T_on TS_1 TS_3 by metis
-  then have TS: "T\<^sub>p_on2 (embed (rTS h)) qs (return_pmf ([x,y],h)) = (length v - 2)" using TS_help by metis
-
-  have splitdet1: "TSdet [x,y] h (u @ v) (length (u @ v))
-      = TSdet (fst (TSdet [x,y] h u (length u))) (rev u @ h) v (length v)" 
-        using splitdet by auto 
-
-  have first: "fst (TSdet [x,y] h u (length u)) = [x,y]"
-    apply(cases "u=[]")
-      apply(simp )
-      using uu by(simp add: rTS_def Step_def TS_step_d_def step_def)
-  
-  have 1: "s_TS [x, y] h qs (length qs) = [y, x]"
-    unfolding s_TS_def qsuv apply(simp only: splitdet1)
-    by(simp only: first inv1[unfolded s_TS_def]) 
-  
-  have TS_inv: "inv_TS qs x y h" unfolding inv_TS_def
-     apply(rule exI[where x="y"])
-     apply(rule exI[where x="x"]) 
-      using 1 inv2 qsuv by(auto) 
-
-  (* BIT *)
-  from BIT_b[OF 2(2,4) vv ] have BITv: "T\<^sub>p_on2 BIT v (type0 init x y) = 3/4 *  ( length v) - 0.5" 
-            and b_c: "config2 BIT v (type0 init x y) (length v) = type0 init y x" by auto
-  from BIT_x[OF 2(2,4) uu] have BITu: "T\<^sub>p_on2 BIT (u @ v) (type0 init x y) = T\<^sub>p_on2 BIT v (type0 init x y)"
-            and x_c: "config2 BIT u (type0 init x y) (length u) = type0 init x y" by auto
-  from BITu BITv have BIT: "T\<^sub>p_on2 BIT qs (type0 init x y) = 0.75 * length v - 0.5"
-        using qsuv  2(4) by auto  
-
-
-  have "config2 BIT (u @ v) (type0 init x y) (length (u @ v)) =
-         config2 BIT v (config2 BIT u (type0 init x y) (length u)) (length v)"
-          by (simp add: config2_append_ge)
-  also have "\<dots> = type0 init y x" by (auto simp add: x_c b_c)
-  finally have config: "config2 BIT qs (type0 init x y) (length qs) = type0 init y x" using qsuv by auto
-  from lenv have "v \<noteq> []"  "last v = y" by auto
-  then have 1:  "last qs = y" using last_appendR qsuv by simp 
-  then have f2: "other (last qs) x y = x" unfolding other_def by simp  
-  
-  from 1 f2 config have BIT_inv: "inv_BIT init qs x y" unfolding inv_BIT_def by auto
-
-  (* OPT *)
-  from uu have u2: "u = [] \<or> u = [x]"  by auto
-  have OPT: "T\<^sub>p [x,y] qs (OPT2 qs [x,y]) = (length v div 2)" using OPT2_B[OF 2(2) qsuv u2 vv] by simp
-
-
-  (* calculation *)
-  have "T\<^sub>p_on2 (COMB h) qs (COMB_state h x y (type0 init x y)) 
-      = 0.2 * T\<^sub>p_on2 (embed (rTS h)) qs (return_pmf ([x,y],h))
-            + 0.8 * T\<^sub>p_on2 BIT qs (type0 init x y)"
-    apply(rule T2_COMB_split)
-      by(simp add: type0_def)
-  also have "\<dots> = 0.2 * (length v - 2) + 0.8 * (0.75 * length v - 0.5)" using TS BIT by simp
-  also have "\<dots> \<le> 1.6 * (length v div 2)"
-  proof -
-    have A: "length v \<ge>2" using lenv by auto
-    have "2 * (length v - 2) + 8 * (0.75 * length v - 0.5)
-          = 8 * length v - 8" using A by(auto simp: ring_distribs)
-    also have "\<dots> \<le> 8*( 2*(length v div 2) +1 ) - 8" by auto
-    also have "\<dots> = 16 * (length v div 2)" by auto
-    finally have 1: "2 * (length v - 2) + 8 * (0.75 * length v - 0.5) \<le> 16 * (length v div 2)" .
-
-    have " 0.2 * (length v - 2) + 0.8 * (0.75 * length v - 0.5)
-        = 1/10 * (2 * (length v - 2) + 8 * (0.75 * length v - 0.5))" by auto
-    also have "\<dots> \<le> 1/10 * (16 * (length v div 2))" using 1 by auto
-    also have "\<dots> = 1.6 * (length v div 2)" by auto
-    finally show ?thesis .
-  qed
-  also have "\<dots> = 1.6 * T\<^sub>p [x, y] qs (OPT2 qs [x, y])" using OPT by simp
-  finally show ?case unfolding inv_COMB_def using BIT_inv TS_inv by auto
-next
-  case 3
-  obtain u v where uu: "u \<in> lang (Plus (Atom x) One)"
-    and vv: "v \<in> lang (seq[Times (Atom y) (Atom x), Star (Times (Atom y) (Atom x)), Atom x])"
-    and qsuv: "qs = u @ v" 
-    using 3
-    by (auto simp: conc_def) 
-
-  have lenv: "length v > 1 \<and> last v = x \<and> v\<noteq>[]"
-  proof -
-    from vv have "v \<in> ({[y]} @@ {[x]}) @@ star({[y]} @@ {[x]}) @@ {[x]}" by(simp add: conc_assoc)
-    then obtain p q r where pqr: "v=p@q@r" and "p\<in>({[y]} @@ {[x]})"
-              and q: "q \<in> star ({[y]} @@ {[x]})" and "r \<in>{[x]}" by (metis concE)
-    then have rr: "p = [y,x]" "r=[x]" by auto
-    with pqr have a: "length v = 3+length q" by auto
-
-    have "last v = last r" using pqr rr by auto
-    then have c: "last v = x" using rr by auto
-    with a show ?thesis by auto
-  qed
-
-
-
-  (* TS *)  
-  from 3(3)[unfolded pre_inv_COMB_def inv_TS_def] obtain x' y' where "x'=x" and "y'=y" 
-      and h: "h=[] \<or> (\<exists>hs. h = [x, x] @ hs)" unfolding s_TS_def by(auto)
-  from TS_xr[OF 3(2) uu h]
-  have  TS_1: "T_TS [x, y] h (u@v) = T_TS [x,y] (rev u @ h) v"
-    and TS_2: "(\<exists>hs. (rev u @ h) = [x, x] @ hs) \<or> (rev u @ h) = [x] \<or> (rev u @ h)=[]" by auto
-  from ts_c[OF 3(2) vv TS_2]
-  have  TS_3: "T_TS [x, y] (rev u @ h) v = (length v - 2)"
-         and  inv1: "s_TS [x,y] (rev u @ h) v (length v) = [x,y]"
-         and  inv2: "(\<exists>hs. (rev v @ (rev u @ h)) = [x,x]@hs)" by auto
-  have "T\<^sub>p_on_rand (embed (rTS h))  [x,y] qs = (length v - 2)"
-    unfolding  qsuv using T_TS_T_on TS_1 TS_3 T_on_embed by metis
-  then have TS: "T\<^sub>p_on2 (embed (rTS h)) qs (return_pmf ([x,y],h)) = (length v - 2)" using TS_help by metis
-
-
-  have splitdet1: "TSdet [x,y] h (u @ v) (length (u @ v))
-      = TSdet (fst (TSdet [x,y] h u (length u))) (rev u @ h) v (length v)" 
-        using splitdet by auto 
-
-  have first: "fst (TSdet [x,y] h u (length u)) = [x,y]"
-    apply(cases "u=[]")
-      apply(simp add:)
-      using uu by(simp add: rTS_def Step_def  TS_step_d_def step_def)
-  
-  have 1: "s_TS [x, y] h qs (length qs) = [x, y]"
-    unfolding s_TS_def qsuv apply(simp only: splitdet1)
-    by(simp only: first inv1[unfolded s_TS_def]) 
-  
-  have TS_inv: "inv_TS qs x y h" unfolding inv_TS_def
-     apply(rule exI[where x="x"])
-     apply(rule exI[where x="y"]) 
-      using 1 inv2 qsuv by(auto) 
-
-  (* BIT *) 
-  from BIT_c[OF 3(2,4) vv] have BITv: "T\<^sub>p_on2 BIT v (type0 init x y) = 0.75 * length v - 0.5" 
-            and c_c: "config2 BIT v (type0 init x y) (length v) = type0 init  x y" by auto
-  from BIT_x[OF 3(2,4) uu] have BITu: "T\<^sub>p_on2 BIT (u @ v) (type0 init x y) = T\<^sub>p_on2 BIT v (type0 init x y)"
-            and x_c: "config2 BIT u (type0 init x y) (length u) = type0 init x y" by auto
-  from BITu BITv have BIT: "T\<^sub>p_on2 BIT qs (type0 init x y) = 0.75 * length v - 0.5"
-        using qsuv by auto
-  
-
-
-  have "config2 BIT (u @ v) (type0 init x y) (length (u @ v)) =
-         config2 BIT v (config2 BIT u (type0 init x y) (length u)) (length v)"
-          by (simp add: config2_append_ge)
-  also have "\<dots> = type0 init x y" by (auto simp add: x_c c_c)
-  finally have config: "config2 BIT qs (type0 init x y) (length qs) = type0 init x y" using qsuv by auto
-  from lenv have "v \<noteq> []"  "last v = x" by auto
-  then have 1:  "last qs = x" using last_appendR qsuv by simp 
-  then have 2: "other (last qs) x y = y" unfolding other_def by simp  
-  
-  from 1 2 config have BIT_inv: "inv_BIT init qs x y" unfolding inv_BIT_def by auto
-
-
-  (* OPT *)
-  from uu have u2: "u = [] \<or> u = [x]"  by auto
-  have OPT: "T\<^sub>p [x,y] qs (OPT2 qs [x,y]) = (length v div 2)" apply(rule OPT2_C) using 3(2) qsuv u2 vv by(simp_all add: conc_assoc)
-
-
-  (* calculation *)  
-  have "T\<^sub>p_on2 (COMB h) qs (COMB_state h x y (type0 init x y)) 
-      = 0.2 * T\<^sub>p_on2 (embed (rTS h)) qs (return_pmf ([x,y],h))
-            + 0.8 * T\<^sub>p_on2 BIT qs (type0 init x y)"
-    apply(rule T2_COMB_split)
-      by(simp add: type0_def)
-  also have "\<dots> = 0.2 * (length v - 2) + 0.8 * (0.75 * length v - 0.5)" using TS BIT by simp
-  also have "\<dots> \<le> 1.6 * (length v div 2)"
-  proof -
-    have A: "length v \<ge>2" using lenv by auto
-    have "2 * (length v - 2) + 8 * (0.75 * length v - 0.5)
-          = 8 * length v - 8" using A by(auto simp: ring_distribs)
-    also have "\<dots> \<le> 8*( 2*(length v div 2) +1 ) - 8" by auto
-    also have "\<dots> = 16 * (length v div 2)" by auto
-    finally have 1: "2 * (length v - 2) + 8 * (0.75 * length v - 0.5) \<le> 16 * (length v div 2)" .
-
-    have " 0.2 * (length v - 2) + 0.8 * (0.75 * length v - 0.5)
-        = 1/10 * (2 * (length v - 2) + 8 * (0.75 * length v - 0.5))" by auto
-    also have "\<dots> \<le> 1/10 * (16 * (length v div 2))" using 1 by auto
-    also have "\<dots> = 1.6 * (length v div 2)" by auto
-    finally show ?thesis .
-  qed
-  also have "\<dots> = 1.6 * T\<^sub>p [x, y] qs (OPT2 qs [x, y])" using OPT by simp
-  finally show ?case unfolding inv_COMB_def using BIT_inv TS_inv by auto
-next
-  case 4
-  then have lqs: "last qs = y" by fastforce
-  from 4(3)[unfolded pre_inv_COMB_def inv_TS_def] obtain x' y' where "x'=x" and "y'=y" 
-      and h: "h=[] \<or> (\<exists>hs. h = [x, x] @ hs)" unfolding s_TS_def by(auto)
-  from ts_a[OF 4(2,5) h]
-  have "real (T_TS [x, y] h qs) = 2" 
-      and TS_inv: "inv_TS qs x y h" by auto
-  then have "T\<^sub>p_on_rand (embed (rTS h)) [x,y] qs = 2"
-      using T_TS_T_on T_on_embed by metis
-  then have TS: "T\<^sub>p_on2 (embed (rTS h)) qs (return_pmf ([x,y],h)) = 2" using TS_help by metis
-
-  have BIT: "T\<^sub>p_on2 BIT qs (type0 init x y) = 1.5" apply(rule BIT_a) using 4 by auto
-  have BIT_inv: "inv_BIT init qs x y" unfolding inv_BIT_def other_def
-    using lqs BIT_a_config[OF 4(1,2,4,5)] by auto
-
-  (* OPT *)
-  have OPT: "T\<^sub>p [x,y] qs (OPT2 qs [x,y]) = 1" using OPT2_A[OF 4(2,5)] by auto
-
-  have "T\<^sub>p_on2 (COMB h) qs (COMB_state h x y (type0 init x y)) 
-      = 0.2 * T\<^sub>p_on2 (embed (rTS h)) qs (return_pmf ([x,y],h))
-            + 0.8 * T\<^sub>p_on2 BIT qs (type0 init x y)"
-    apply(rule T2_COMB_split)
-      by(simp add: type0_def)
-  also have "\<dots> = 1.6" using TS BIT by simp
-  also have "\<dots> \<le> 1.6 * T\<^sub>p [x, y] qs (OPT2 qs [x, y])" using OPT by simp
-  finally show ?case unfolding inv_COMB_def using BIT_inv TS_inv by auto
-qed simp
-    
-
-lemma config2_COMB: "i<length qs \<Longrightarrow> config2 (COMB h1) qs initdistr i = config2 (COMB h2) qs initdistr i"
-apply(induct i) by(simp_all add: COMB_def config2_def take_Suc_conv_app_nth config'_rand_append)
-
-lemma h_indifferent: "T\<^sub>p_on2 (COMB h1) qs initdistr = T\<^sub>p_on2 (COMB h2) qs initdistr"
-unfolding T\<^sub>p_on2_def
-  apply(rule setsum.cong)
-    apply(simp)
-     unfolding T_on_n2_def
-     apply(simp)
-     apply(subst config2_COMB[of _ _ _ _ h2, unfolded config2_def]) by (simp_all add: COMB_def) 
-            
-theorem COMB_OPT2: "(x::nat) \<noteq> y
-     \<Longrightarrow> pre_inv_COMB init x y h
-     \<Longrightarrow> init\<in>{[x,y],[y,x]}
-     \<Longrightarrow> set \<sigma> \<subseteq> {x,y}
-     \<Longrightarrow> T\<^sub>p_on2 (COMB h) \<sigma> (COMB_state h x y (type0 init x y)) \<le> 1.6 * T\<^sub>p [x,y] \<sigma> (OPT2 \<sigma> [x,y]) + 2"
- proof (induction "length \<sigma>" arbitrary: \<sigma> x y h rule: less_induct)
-  case (less \<sigma>)
-  let ?initstate = "(COMB_state h x y (type0 init x y))" 
+          apply(simp) apply(simp)  
+          apply(simp add: set_pmf_bernoulli)
+          apply(simp add: BIT_step_def COMB_def COMB_step_def split_def)
+          apply(safe) 
+            using BIT_config'_fin[OF assms(2)] apply(simp)
+            using TS_config'_fin[OF assms(3)] apply(simp)
+          apply(simp)
+      apply(simp only: map_pmf_def[where f=Inl])
+      apply(simp only: map_pmf_def[where f=Inr])
+        apply(simp add: bind_return_pmf bind_assoc_pmf COMB_def COMB_step_def)
+        apply(simp add: split_def)
+        apply(simp add: rTS_def map_pmf_def bind_return_pmf bind_assoc_pmf COMB_def COMB_step_def)
+              
+    done
 
   show ?case
-  proof (cases "\<exists>xs ys. \<sigma>=xs@ys \<and> xs \<in> Lxx x y")
-    case True 
+    apply(simp only: T_on_rand'_append)
+    apply(subst snoc)
+    apply(subst P) by algebra 
 
-    then obtain xs ys where qs: "\<sigma>=xs@ys" and xsLxx: "xs \<in> Lxx x y" by auto
+qed simp
 
-    with Lxx1 have len: "length ys < length \<sigma>" by fastforce
-    from qs(1) less(5) have ysxy: "set ys \<subseteq> {x,y}" by auto
-
-
-    have xsset: "set xs \<subseteq> {x, y}" using less(5) qs by auto
-    from xsLxx Lxx1 have lxsgt1: "length xs \<ge> 2" by auto
-    then have xs_not_Nil: "xs \<noteq> []" by auto
-
-    from D[OF xsLxx less(2-4)]
-      have D1: "T\<^sub>p_on2 (COMB h) xs (COMB_state h x y (type0 init x y)) \<le> 1.6 * T\<^sub>p [x, y] xs (OPT2 xs [x, y])" 
-         and invCOMB: "inv_COMB init xs x y h" by auto
-
-    from invCOMB[unfolded inv_COMB_def inv_TS_def inv_BIT_def]
-      have invBIT: "config2 BIT xs (type0 init x y) (length xs) = type0 init (last xs) (other (last xs) x y)" 
-      and invTS: "(\<exists>x' y'. s_TS [x, y] h xs (length xs) = [x', y'] \<and> (\<exists>hs. rev xs @ h = [x', x'] @ hs))" by auto
- 
-     have "s_TS [x, y] h xs (length xs) = [last xs, other (last xs) x y]"
-        and invTS_2: "(\<exists>hs. rev xs @ h = [last xs, last xs] @ hs)"  
-        and invTS_config2: "config2 (embed (rTS h)) xs (return_pmf ([x, y], h)) (length xs)
-            = return_pmf ([last xs, other (last xs) x y], rev xs@h)"
-      proof (goal_cases)
-        from invTS obtain x' y' hs where f1: "s_TS [x, y] h xs (length xs) = [x', y']"
-                and h: "rev xs @ h = [x', x'] @ hs" by auto
-        have "hd (rev xs @ h) = x'" using h by auto
-        with xs_not_Nil have "hd (rev xs) = x'" by(auto)
-        with xs_not_Nil hd_rev have xlast: "x' = last xs" by metis
-        from s_TS_xy[OF less(2) xsset, of "length xs" h] less(2) f1 have
-            xyxy: "[x', y'] \<in> {[x,y], [y,x]}" by force
-        have "x'\<noteq>y'" and "(x'=x \<and> y'=y) \<or> (x'=y \<and> y'=x)"
-            using xyxy less(2) by auto
-        then have yother: "y' = other x' x y" unfolding other_def by auto
-        case 1
-        show fstTS: ?case using f1 xlast yother by auto
-        case 2
-        show ?case using h xlast by auto
-        case 3
-        have sndTS: "snd (TSdet [x,y] h xs (length xs)) = (rev xs)@h"
-          apply(subst sndTSdet) by(auto)
- 
-        have "config2 (embed (rTS h)) xs (return_pmf ([x, y], h)) (length xs) 
-              = config'' (embed (rTS h)) xs [x,y] (length xs)"
-          unfolding rTS_def config2_def by(simp add: bind_return_pmf)
-        also have "\<dots> =  (return_pmf ( TSdet [x,y] h xs (length xs)))"
-             apply(subst config_embed) by simp
-        also have "\<dots> = return_pmf ([last xs, other (last xs) x y], rev xs@h)"
-          using sndTS fstTS[unfolded s_TS_def]  apply(cases " TSdet [x,y] h xs (length xs)")
-            by(simp) 
-        finally  show ?case .
-    qed
-
-    from xsLxx Lxx_ends_in_two_equal obtain pref e where "xs = pref @ [e,e]" by metis
-    then have endswithsame: "xs = pref @ [last xs, last xs]" by auto 
-
-    let ?c' = "[last xs, other (last xs) x y]" 
-
-    have setys: "set ys \<subseteq> {x,y}" using qs less by auto 
-    have setxs: "set xs \<subseteq> {x,y}" using qs less by auto 
-    have lxs: "last xs \<in> set xs" using xs_not_Nil by auto
-    from lxs setxs have lxsxy: "last xs \<in> {x,y}" by auto 
-     from lxs setxs have otherxy: "other (last xs) x y \<in> {x,y}" by (simp add: other_def)
-    from less(2) have other_diff: "last xs \<noteq> other (last xs) x y" by(simp add: other_def)
- 
-    have nextstate: "{[last xs, other (last xs) x y], [other (last xs) x y, last xs]}
-            = { [x,y],[y,x]}" using lxsxy otherxy other_diff by fastforce
-    have setys': "set ys \<subseteq> {last xs, other (last xs) x y}"
-            using setys lxsxy otherxy other_diff by fastforce
-
-    let ?nextstate = "(COMB_state (rev xs @ h) (last xs) (other (last xs) x y) (type0 init (last xs) (other (last xs) x y)))"
-
-    have yeaah: "config2 (COMB h) xs ?initstate (length xs)  = ?nextstate"
-      apply(subst config2COMB)
-        apply(simp)
-        apply(subst invBIT) 
-        apply(subst invTS_config2)
-        unfolding COMB_state_def by(simp add: bind_return_pmf)  
-
-    have "T\<^sub>p_on2 (COMB h)  ys (config2 (COMB h)  xs ?initstate (length xs))
-        = T\<^sub>p_on2 (COMB h)  ys ?nextstate"
-          by(simp only: yeaah)  
-    also have "\<dots> = T\<^sub>p_on2 (COMB (rev xs @ h))  ys ?nextstate"
-      using h_indifferent by auto
-    also from len have "\<dots> \<le> 1.6 * T\<^sub>p ?c' ys (OPT2 ys ?c') + 2"       
-            apply(rule less(1))
-              using less(2) apply(simp add: other_def)
-              unfolding pre_inv_COMB_def using invTS_2 apply(simp) 
-              using less(4) nextstate apply(simp) 
-              by(fact setys')
-     finally have c: "T\<^sub>p_on2 (COMB h)  ys (config2 (COMB h)  xs ?initstate (length xs))
-                  \<le> 1.6 * T\<^sub>p ?c' ys (OPT2 ys ?c') + 2" .
-
-
-    have well: "T\<^sub>p [x, y] xs (OPT2 xs [x, y]) + T\<^sub>p ?c' ys (OPT2 ys ?c')
-        = T\<^sub>p [x, y] (xs @ ys) (OPT2 (xs @ ys) [x, y])"
-          apply(rule OPTauseinander[where pref=pref])
-            apply(fact)+
-            using lxsxy other_diff otherxy apply(fastforce)
-            apply(simp)
-            using endswithsame by simp  
-
-    have E0: " T\<^sub>p_on2 (COMB h) \<sigma> ?initstate
-          =  T\<^sub>p_on2 (COMB h) (xs@ys) ?initstate" using qs by auto
-     also have E1: "\<dots> = T\<^sub>p_on2 (COMB h) xs ?initstate
-              + T\<^sub>p_on2 (COMB h)  ys (config2 (COMB h)  xs ?initstate (length xs))"
-      unfolding COMB_def  by (rule splitquerylist2)
-    also have E2: "\<dots> \<le> T\<^sub>p_on2 (COMB h) xs ?initstate + 1.6 * T\<^sub>p ?c' ys (OPT2 ys ?c') + 2"
-        using c by simp
-    also have E3: "\<dots> \<le> 1.6 * T\<^sub>p [x, y] xs (OPT2 xs [x, y]) + 1.6 * T\<^sub>p ?c' ys (OPT2 ys ?c') + 2"
-        using D1 by simp        
-    also have "\<dots> \<le> 1.6 * (T\<^sub>p [x,y] xs (OPT2 xs [x,y]) + T\<^sub>p ?c' ys (OPT2 ys ?c')) + 2"
-        by(auto)
-    also have  "\<dots> = 1.6 * (T\<^sub>p [x,y] (xs@ys) (OPT2 (xs@ys) [x,y])) + 2"
-      using well by auto 
-    also have E4: "\<dots> = 1.6 * (T\<^sub>p [x,y] \<sigma> (OPT2 \<sigma> [x,y])) + 2"
-        using qs by auto
-    finally show ?thesis .
- 
-
-  next
-    case False
-    note f1=this
-    from Lxx_othercase[OF less(5) this, unfolded hideit_def] have
-        nodouble: "\<sigma> = [] \<or> \<sigma> \<in> lang (nodouble x y)" by  auto
-    show ?thesis
-    proof (cases "\<sigma> = []")
-      case True
-      then show ?thesis unfolding T\<^sub>p_on2_def  by(simp)
-    next
-      case False
-      (* with padding *)
-      from False nodouble have qsnodouble: "\<sigma> \<in> lang (nodouble x y)" by auto
-      let ?padded = "pad \<sigma> x y"
-      from False pad_adds2[of \<sigma> x y] less(5) obtain addum where ui: "pad \<sigma> x y = \<sigma> @ [last \<sigma>]" by auto
-      from nodouble_padded[OF False qsnodouble] have pLxx: "?padded \<in> Lxx x y" .
-
-      have E0: "T\<^sub>p_on2 (COMB h) \<sigma> ?initstate \<le> T\<^sub>p_on2 (COMB h) ?padded ?initstate"
-      proof -
-        have "T\<^sub>p_on2 (COMB h) \<sigma> ?initstate = setsum (T_on_n2 (COMB h) \<sigma> ?initstate) {..<length \<sigma>}"
-          unfolding T\<^sub>p_on2_def by simp
-        also have "\<dots>
-             = setsum (T_on_n2 (COMB h) (\<sigma> @ [last \<sigma>]) ?initstate) {..<length \<sigma>}"
-          proof(rule setsum.cong, goal_cases)
-            case (2 t)
-            then have "t < length \<sigma>" by auto 
-            then show ?case unfolding T_on_n2_def by(simp add: nth_append)
-          qed simp
-        also have "... \<le> T\<^sub>p_on2 (COMB h) ?padded ?initstate"
-          unfolding ui T\<^sub>p_on2_def apply(simp)
-          unfolding COMB_def T_on_n2_def by(simp only: T_on_rand'_nn) 
-        finally show ?thesis by auto
-      qed  
-
-      also from pLxx have E1: "\<dots> \<le> 1.6 * T\<^sub>p [x,y] ?padded (OPT2 ?padded [x,y])"
-        using D[OF pLxx less(2-4) ] by simp
-      also have E2: "\<dots> \<le> 1.6 * T\<^sub>p [x,y] \<sigma> (OPT2 \<sigma> [x,y]) + 2"
-      proof -
-        from False less(2) obtain \<sigma>' x' y' where qs': "\<sigma> = \<sigma>' @ [x']" and x': "x' = last \<sigma>" "y'\<noteq>x'" "y' \<in>{x,y}" 
-            by (metis append_butlast_last_id insert_iff)
-        have tla: "last \<sigma> \<in> {x,y}" using less(5) False last_in_set by blast
-        with x' have grgr: "{x,y} = {x',y'}" by auto
-        then have "(x = x' \<and> y = y') \<or> (x = y' \<and> y = x')" using less(2) by auto
-        then have tts: "[x, y] \<in> {[x', y'], [y', x']}" by blast
-        
-        from qs' ui have pd: "?padded = \<sigma>' @ [x', x']" by auto 
-
-        have "T\<^sub>p [x,y] (?padded) (OPT2 (?padded) [x,y])
-              = T\<^sub>p [x,y] (\<sigma>' @ [x', x']) (OPT2 (\<sigma>' @ [x', x']) [x,y])"
-                unfolding pd by simp
-        also have gr: "\<dots>
-            \<le> T\<^sub>p [x,y] (\<sigma>' @ [x']) (OPT2 (\<sigma>' @ [x']) [x,y]) + 1"
-              apply(rule OPT2_padded[where x="x'" and y="y'"])
-                apply(fact)
-                using grgr qs' less(5) by auto
-        also have "\<dots> \<le> T\<^sub>p [x,y] (\<sigma>) (OPT2 (\<sigma>) [x,y]) + 1" 
-              unfolding qs' by simp
-        finally show ?thesis by auto
-      qed
-      finally show ?thesis .  
-    qed
-  qed 
-qed  
-
-
-theorem COMB_on2: assumes
- "set \<sigma> \<subseteq> {x,y}" and  "(x::nat) \<noteq> y"
-  shows
-      "T\<^sub>p_on_rand (COMB []) [x,y] \<sigma>  \<le> 1.6 * T\<^sub>p_opt [x, y] \<sigma> + 2"
+lemma Combination:
+  assumes "qs \<in> pattern" "a \<noteq> b" "{a, b} = {x, y}" "set qs \<subseteq> {a, b}"
+    and "inv_COMB s a [x,y]"
+    and TS: "\<And>s h. a \<noteq> b \<Longrightarrow> {a, b} = {x, y} \<Longrightarrow> TS_inv s a [x, y] \<Longrightarrow> set qs \<subseteq> {a, b}
+      \<Longrightarrow> qs \<in> pattern \<Longrightarrow>
+            TS_inv (config'_rand (embed (rTS h)) s qs) (last qs) [x, y] 
+          \<and> T\<^sub>p_on_rand' (embed (rTS h)) s qs = ts"
+    and BIT: "\<And>s. a \<noteq> b \<Longrightarrow> {a, b} = {x, y} \<Longrightarrow> BIT_inv s a [x, y] \<Longrightarrow> set qs \<subseteq> {a, b}
+      \<Longrightarrow> qs \<in> pattern \<Longrightarrow>
+            BIT_inv (config'_rand BIT s qs) (last qs) [x, y] 
+          \<and> T\<^sub>p_on_rand' BIT s qs = bit"
+    and OPT_cost: "a \<noteq> b \<Longrightarrow> qs \<in> pattern \<Longrightarrow> real (T\<^sub>p [a, b] qs (OPT2 qs [a, b])) = opt"
+    and absch: "qs \<in> pattern \<Longrightarrow> 0.2 * ts + 0.8 * bit \<le> 1.6 * opt"
+  shows "T\<^sub>p_on_rand' (COMB []) s qs \<le> 16 / 10 * real (T\<^sub>p [a, b] qs (OPT2 qs [a, b])) \<and>
+    inv_COMB (Partial_Cost_Model.config'_rand (COMB []) s qs) (last qs) [x, y]"
 proof -
-  have pre: "pre_inv_COMB [x,y] x y []" unfolding pre_inv_COMB_def by simp
+  let ?D = "map_pmf con s"
+  from assms(5) obtain Da Db where Daf: "finite (set_pmf Da)"
+      and Dbf: "finite (set_pmf Db)"
+      and D: "?D = Sum_pmf 0.8 Da Db"
+             and B: "BIT_inv Da a [x,y]" and T: "TS_inv Db a [x,y]"
+    unfolding inv_COMB_def by auto 
+     
 
-  have "T\<^sub>p_on_rand (COMB []) [x,y] \<sigma> = 
-         T\<^sub>p_on2 (COMB []) \<sigma> (COMB_state [] x y (type0 [x,y] x y))"
-         unfolding T\<^sub>p_on2_def T_on_rand_as_sum T_on_n2_def COMB_state_def COMB_def
-         apply(rule setsum.cong)
-          apply(simp)
-          apply(simp add: type0_def bind_return_pmf bind_assoc_pmf)
-          apply(rule arg_cong[where f=E])
-          apply(rule bind_pmf_cong)
-            apply(simp_all)
-            apply(rule arg_cong2[where f="config'_rand (COMB_init [], COMB_step)"])
-              apply(rule bind_pmf_cong)
-                apply(simp add: set_pmf_bernoulli)
-                  apply(case_tac xaa)
-                    apply(simp) using bind_commute_pmf apply fast
-                    apply(simp)               
-              apply(simp)
-         done
-  also have "\<dots> \<le> 1.6 * T\<^sub>p [x,y] \<sigma> (OPT2 \<sigma> [x,y]) + 2"
-    apply(rule COMB_OPT2)
-      using assms pre by (simp_all)
-  also have "\<dots> = 1.6 * T\<^sub>p_opt [x, y] \<sigma> + 2"
-    using OPT2_is_opt[OF assms] by(simp)
-  finally show ?thesis .
+  let ?Da' = "config'_rand BIT Da qs"
+  from BIT[OF assms(2,3) B assms(4,1) ]
+    have B': "BIT_inv ?Da' (last qs) [x, y]"
+    and B_cost: "T\<^sub>p_on_rand' BIT Da qs = bit" by auto
+
+  let ?Db' = "config'_rand (embed (rTS [])) Db qs"
+  (* ähnlich *) 
+  from TS[OF assms(2,3) T assms(4,1)] 
+    have T': "TS_inv ?Db' (last qs) [x, y]"
+    and T_cost: "T\<^sub>p_on_rand' (embed (rTS [])) Db qs = ts" by auto 
+
+  have "T\<^sub>p_on_rand' (COMB []) s qs
+        = 0.2 * T\<^sub>p_on_rand' (embed (rTS [])) Db qs
+            + 0.8 * T\<^sub>p_on_rand' BIT Da qs" 
+         using D apply(rule obligation2) apply(fact Daf) apply(fact Dbf) done
+also
+  have "\<dots>  \<le> 1.6 * opt"
+    by (simp only: B_cost T_cost absch[OF assms(1)])
+also
+  have "\<dots> = 1.6 * T\<^sub>p [a, b] qs (OPT2 qs [a, b])" by (simp add: OPT_cost[OF assms(2,1)]) 
+finally
+  have Comb_cost: "T\<^sub>p_on_rand' (COMB []) s qs \<le> 1.6 * T\<^sub>p [a, b] qs (OPT2 qs [a, b])" .
+
+  have Comb_inv: "inv_COMB (config'_rand (COMB []) s qs) (last qs) [x, y]"
+      unfolding inv_COMB_def
+      apply(rule exI[where x="?Da'"])
+      apply(rule exI[where x="?Db'"])
+        apply(safe)
+          apply(rule BIT_config'_fin[OF Daf])
+          apply(rule TS_config'_fin[OF Dbf])
+          apply(rule obligation1)
+          apply(fact D)
+          apply(fact B')
+          apply(fact T') done
+
+  from Comb_cost Comb_inv show ?thesis by simp
 qed
 
+theorem COMB_OPT2':  "(x::nat) \<noteq> y \<Longrightarrow> set \<sigma> \<subseteq> {x,y}
+     \<Longrightarrow> T\<^sub>p_on_rand (COMB []) [x,y] \<sigma>  \<le> 1.6 * real (T\<^sub>p_opt [x,y] \<sigma>) + 1.6"
+proof (rule Phase_partitioning_general[where P="inv_COMB"], goal_cases)
+  case 4
+  let ?initBIT ="(map_pmf (Pair [x, y]) (fst BIT [x, y]))"
+  let ?initTS ="(map_pmf (Pair [x, y]) (fst (embed (rTS [])) [x, y]))"
+  show  "inv_COMB (map_pmf (Pair [x, y]) (fst (COMB []) [x, y])) x [x, y]" 
+    unfolding inv_COMB_def
+    apply(rule exI[where x="?initBIT"])
+    apply(rule exI[where x="?initTS"])
+      apply(simp only: BIT_inv_initial[OF 4(1)] )
+      apply(simp add: map_pmf_def bind_return_pmf bind_assoc_pmf COMB_def)
+      apply(simp add: Sum_pmf_def)
+     apply(safe)
+         apply(simp add: BIT_init_def)
+        apply(rule bind_pmf_cong)
+          apply(simp)
+          apply(simp add: bind_return_pmf bind_assoc_pmf rTS_def map_pmf_def BIT_init_def)
+       apply(simp add: TS_inv_def rTS_def)    
+      done
+next
+  case (5 a b qs s)
+  from 5(3)
+  show ?case
+    proof (rule LxxE, goal_cases)
+      case 4
+      then show ?thesis apply(rule Combination)
+        apply(fact)+
+        using TS_a'' apply(simp)
+        apply(fact bit_a'')
+        apply(fact OPT2_A')
+        apply(simp)
+      done
+    next
+      case 1
+      then show ?case
+        apply(rule Combination)
+        apply(fact)+
+        apply(fact TS_d'') 
+        apply(fact bit_d')
+        by auto
+    next
+      case 2
+      then have "qs \<in> lang (seq [Atom b, Atom a, Star (Times (Atom b) (Atom a)), Atom b, Atom b])
+              \<or> qs \<in> lang (seq [Atom a, Atom b, Atom a, Star (Times (Atom b) (Atom a)), Atom b, Atom b])" by auto
+      then show ?case
+        apply(rule disjE)
+          apply(erule Combination)
+            apply(fact)+
+            apply(fact TS_b1'') 
+            apply(fact bit_b''1) 
+            apply(fact OPT2_B1)
+            apply(simp add: ring_distribs)
+         apply(erule Combination)
+           apply(fact)+
+           apply(fact TS_b2'') 
+           apply(fact bit_b''2) 
+           apply(fact OPT2_B2)
+           apply(simp add: ring_distribs)
+        done
+    next
+      case 3
+      then have len: "length qs \<ge> 2" by(auto simp add: conc_def)
+      have len2: "qs \<in> lang (seq [Atom a, Atom b, Atom a, Star (Times (Atom b) (Atom a)), Atom a]) 
+                  \<Longrightarrow> length qs \<ge> 3" by (auto simp add: conc_def)
+      from 3 have "qs \<in> lang (seq [Atom b, Atom a, Star (Times (Atom b) (Atom a)), Atom a])
+              \<or> qs \<in> lang (seq [Atom a, Atom b, Atom a, Star (Times (Atom b) (Atom a)), Atom a])" by auto
+      then show ?case
+        apply(rule disjE)
+          apply(erule Combination)
+            apply(fact)+
+            apply(fact TS_c1'')
+            apply(fact bit_c''1)  
+            apply(fact OPT2_C1)
+            using len apply(simp add: ring_distribs)
+         apply(erule Combination)
+           apply(fact)+
+           apply(fact TS_c2'')
+           apply(fact bit_c''2)
+           apply(fact OPT2_C2)
+           using len2 apply(simp add: ring_distribs conc_def)
+        done
+    qed
+qed (simp_all) 
 
 
-
-
-subsubsection "COMB pairwise"
-
+section "COMB pairwise"
 
 lemma config_rand_COMB: "config_rand (COMB h) init qs = do {
                     (b::bool) \<leftarrow> (bernoulli_pmf 0.8); 
                     (b1,b2) \<leftarrow>  (config_rand BIT init qs);
                     (t1,t2) \<leftarrow>  (config_rand (embed (rTS h)) init qs);
-                    return_pmf (if b then  (b1, CBit b2) else (t1, CTs t2))
+                    return_pmf (if b then  (b1, Inl b2) else (t1, Inr t2))
                     }" (is "?LHS = ?RHS")
 proof (induct qs rule: rev_induct)
   case Nil
@@ -747,6 +349,12 @@ next
             apply(case_tac x)
                by(simp_all add: COMB_def COMB_step_def rTS_def map_pmf_def split_def bind_return_pmf bind_assoc_pmf)
 qed
+
+lemma COMB_no_paid: " \<forall>((free, paid), t)\<in>set_pmf (snd (COMB []) (s, is) q). paid = []"
+apply(simp add:  COMB_def COMB_step_def split_def BIT_step_def TS_step_d_def)
+apply(case_tac "is")
+  by(simp_all add: BIT_step_def TS_step_d_def)
+  
 
 lemma COMB_pairwise: "pairwise (COMB [])"
 proof(rule pairwise_property_lemma, goal_cases) 
@@ -772,49 +380,27 @@ proof(rule pairwise_property_lemma, goal_cases)
 next
   case (2 xa r)
   show ?case
-    apply(simp add: COMB_def COMB_step_def split_def)
-    apply(case_tac "snd xa")
-      by(simp_all add: BIT_step_def TS_step_d_def)
+    using COMB_no_paid
+    by (metis (mono_tags) case_prod_unfold surj_pair)  
 qed 
           
 
-subsubsection "COMB 1.6-competitive"
-
-
+section "COMB 1.6-competitive"
 
 lemma finite_config_TS: "finite (set_pmf (config'' (embed (rTS h)) qs init n))" (is "finite ?D")
   apply(subst config_embed)
-    by(simp)
+    by(simp) 
 
 lemma COMB_has_finite_config_set: assumes [simp]: "distinct init"
-      and "set qs \<subseteq> set init"
-      and "x<length qs"
-      shows "finite (set_pmf (config'' (COMB h) qs init x))"
-proof -
+      and "set qs \<subseteq> set init" 
+      shows "finite (set_pmf (config_rand (COMB h) init qs))"
+proof - 
+  from finite_config_TS[where n="length qs" and qs=qs]
+      finite_config_BIT[OF assms(1)] 
   show ?thesis 
-      apply(subst configCOMB)
-        using assms(3) apply(simp)
-        apply(subst set_bind_pmf)
-          apply(simp only: set_pmf_bernoulli split_def)
-          apply(rule finite_UN_I)
-            apply(simp)
-            apply(case_tac M)
-              apply(simp)
-              apply(rule finite_UN_I)
-                using finite_config_BIT[OF assms(1)] apply auto[1]
-                apply(simp)
-              apply(simp)
-              apply(rule finite_UN_I) 
-                using finite_config_TS  apply auto[1]
-                by simp
+    apply(subst obligation1'')
+      by(simp add: Sum_pmf_def)  
 qed
-
-lemma COMB_no_paid: " \<forall>((free, paid), t)\<in>set_pmf (snd (COMB []) (s, is) q). paid = []"
-apply(simp add:  COMB_def COMB_step_def split_def BIT_step_def TS_step_d_def)
-apply(case_tac "is")
-  by(simp_all add: BIT_step_def TS_step_d_def)
-  
-
 
 theorem COMB_competitive: "\<forall>s0\<in>{x::nat list. distinct x \<and> x\<noteq>[]}.
    \<exists>b\<ge>0. \<forall>qs\<in>{x. set x \<subseteq> set s0}.
@@ -862,15 +448,16 @@ proof(rule factoringlemma_withconstant, goal_cases)
             
             show ?case
               apply(cases "(Lxy init {a, b}) = [a,b]")  
-                apply(simp) using COMB_on2[OF b1 a] apply(simp)
+                apply(simp) using COMB_OPT2'[OF a b1] a apply(simp)
                 using pos apply(simp) unfolding twist 
-              using COMB_on2[OF b2 a[symmetric]] by(simp)
+              using COMB_OPT2'[OF a[symmetric] b2] by simp
           qed
     qed
 next
   case 4  then show ?case using COMB_pairwise by simp
 next
-  case 7 then show ?case using COMB_has_finite_config_set[unfolded MTF_def, OF 7] by simp
+  case 7 then show ?case apply(subst COMB_has_finite_config_set[OF 7(1)])
+        using set_take_subset apply fast by simp
 qed (simp_all add: COMB_no_paid)
 
 
